add avx512 intrinsics and transpose16x16

lib/c/libintvector.h
@@ -377,6 +377,127 @@ typedef __m256i Lib_IntVector_Intrinsics_vec256;
 #define Lib_IntVector_Intrinsics_vec256_interleave_high128(x1, x2) \
   (_mm256_permute2x128_si256(x1, x2, 0x31))
 
+
+typedef __m512i Lib_IntVector_Intrinsics_vec512;
+
+#define Lib_IntVector_Intrinsics_vec512_zero  \
+  (_mm512_setzero_epi32())
+
+#define Lib_IntVector_Intrinsics_vec512_load32s(x0,x1,x2,x3,x4,x5,x6,x7,x8,x9,x10,x11,x12,x13,x14,x15) \
+  (_mm512_set_epi32(x15,x14,x13,x12,x11,x10,x9,x8,x7,x6,x5,x4,x3,x2,x1,x0)) /* hi lo */
+
+#define Lib_IntVector_Intrinsics_vec512_load64s(x0,x1,x2,x3,x4,x5,x6,x7) \
+  (_mm512_set_epi64(x7,x6,x5,x4,x3,x2,x1,x0)) /* hi lo */
+
+#define Lib_IntVector_Intrinsics_vec512_load32(x) \
+  (_mm512_set1_epi32(x))
+
+#define Lib_IntVector_Intrinsics_vec512_load64(x) \
+  (_mm512_set1_epi64(x))
+
+#define Lib_IntVector_Intrinsics_vec512_insert32(x0, x1, x2) \
+  (x2<8? _mm512_inserti32x8(x0,_mm256_insert_epi32(_mm512_extracti32x8_epi32(x0,0),x1,x2),0) : _mm512_inserti32x8(x0,_mm256_insert_epi32(_mm512_extracti32x8_epi32(x0,1),x1,x2-8),1)) //TODO : FIX!
+
+#define Lib_IntVector_Intrinsics_vec512_extract32(x0, x1) \
+  (x1<8? _mm256_extract_epi32(_mm512_extracti32x8_epi32(x0,0),x1) : _mm256_extract_epi32(_mm512_extracti32x8_epi32(x0,1),x1-8)) //TODO : FIX!
+
+#define Lib_IntVector_Intrinsics_vec512_insert64(x0, x1, x2) \
+  (x2<4? _mm512_inserti64x4(x0,_mm256_insert_epi64(_mm512_extracti64x4_epi64(x0,0),x1,x2),0) : _mm512_inserti64x4(x0,_mm256_insert_epi64(_mm512_extracti64x4_epi64(x0,1),x1,x2-4),1)) //TODO : FIX!
+
+#define Lib_IntVector_Intrinsics_vec512_extract64(x0, x1) \
+  (x1<4? _mm256_extract_epi64(_mm512_extracti64x4_epi64(x0,0),x1) : _mm256_extract_epi64(_mm512_extracti64x4_epi64(x0,1),x1-4)) //TODO : FIX!
+
+#define Lib_IntVector_Intrinsics_vec512_add32(x0, x1) \
+  (_mm512_add_epi32(x0, x1))
+
+#define Lib_IntVector_Intrinsics_vec512_add64(x0, x1) \
+  (_mm512_add_epi64(x0, x1))
+
+#define Lib_IntVector_Intrinsics_vec512_sub32(x0, x1) \
+  (_mm512_sub_epi32(x0, x1))
+
+#define Lib_IntVector_Intrinsics_vec512_sub64(x0, x1) \
+  (_mm512_sub_epi64(x0, x1))
+
+#define Lib_IntVector_Intrinsics_vec512_mul32(x0, x1) \
+  (_mm512_mul_epu32(x0, x1))
+
+#define Lib_IntVector_Intrinsics_vec512_mul64(x0, x1) \
+  (_mm512_mul_epu32(x0, x1))
+
+#define Lib_IntVector_Intrinsics_vec512_smul32(x0, x1) \
+  (_mm512_mul_epu32(x0, _mm512_set1_epi32(x1)))
+
+#define Lib_IntVector_Intrinsics_vec512_smul64(x0, x1) \
+  (_mm512_mul_epu32(x0, _mm512_set1_epi64(x1)))
+
+#define Lib_IntVector_Intrinsics_vec512_xor(x0, x1) \
+  (_mm512_xor_si512(x0, x1))
+
+#define Lib_IntVector_Intrinsics_vec512_and(x0, x1) \
+  (_mm512_and_si512(x0, x1))
+
+#define Lib_IntVector_Intrinsics_vec512_or(x0, x1) \
+  (_mm512_or_si512(x0, x1))
+
+#define Lib_IntVector_Intrinsics_vec512_lognot(x0) \
+  (_mm512_xor_si512(x0, _mm512_set1_epi32(-1)))
+
+#define Lib_IntVector_Intrinsics_vec512_shift_left32(x0, x1) \
+  (_mm512_slli_epi32(x0, x1))
+
+#define Lib_IntVector_Intrinsics_vec512_shift_left64(x0, x1) \
+  (_mm512_slli_epi64(x0, x1))
+
+#define Lib_IntVector_Intrinsics_vec512_shift_right32(x0, x1) \
+  (_mm512_srli_epi32(x0, x1))
+
+#define Lib_IntVector_Intrinsics_vec512_shift_right64(x0, x1) \
+  (_mm512_srli_epi64(x0, x1))
+
+#define Lib_IntVector_Intrinsics_vec512_rotate_left32(x0, x1) \
+  (_mm512_rol_epi32(x0, x1))
+
+#define Lib_IntVector_Intrinsics_vec512_rotate_left64(x0, x1) \
+  (_mm512_rol_epi64(x0, x1))
+
+#define Lib_IntVector_Intrinsics_vec512_eq64(x0, x1) \
+  (_mm512_maskz_broadcastq_epi64(_mm512_cmpeq_epi64_mask(x0, x1), _mm_set1_epi8(0xFF))) //TODO : FIX!
+
+#define Lib_IntVector_Intrinsics_vec512_gt64(x0, x1) \
+  (_mm512_maskz_broadcastq_epi64(_mm512_cmpgt_epi64_mask(x0, x1), _mm_set1_epi8(0xFF))) //TODO : FIX!
+
+#define Lib_IntVector_Intrinsics_vec512_load_le(x0) \
+  (_mm512_loadu_si512((__m512i*)(x0)))
+
+#define Lib_IntVector_Intrinsics_vec512_store_le(x0, x1) \
+  (_mm512_storeu_si512((__m512i*)(x0), x1))
+
+#define Lib_IntVector_Intrinsics_vec512_interleave_low32(x1, x2) \
+  (_mm512_unpacklo_epi32(x1, x2))
+
+#define Lib_IntVector_Intrinsics_vec512_interleave_high32(x1, x2) \
+  (_mm512_unpackhi_epi32(x1, x2))
+
+#define Lib_IntVector_Intrinsics_vec512_interleave_low64(x1, x2) \
+  (_mm512_unpacklo_epi64(x1, x2))
+
+#define Lib_IntVector_Intrinsics_vec512_interleave_high64(x1, x2) \
+  (_mm512_unpackhi_epi64(x1, x2))
+
+#define Lib_IntVector_Intrinsics_vec512_interleave_low128(x1, x2)	\
+  (_mm512_permutex2var_epi64(x1, _mm512_set_epi64(13,12,5,4,9,8,1,0), x2))
+
+#define Lib_IntVector_Intrinsics_vec512_interleave_high128(x1, x2) \
+  (_mm512_permutex2var_epi64(x1, _mm512_set_epi64(15,14,7,6,11,10,3,2), x2))
+
+#define Lib_IntVector_Intrinsics_vec512_interleave_low256(x1, x2) \
+  (_mm512_shuffle_i32x4(x1, x2, 0x44))
+
+#define Lib_IntVector_Intrinsics_vec512_interleave_high256(x1, x2) \
+  (_mm512_shuffle_i32x4(x1, x2, 0xee))
+
+
 #elif defined(__aarch64__) || defined(_M_ARM64) || defined(__arm__) || defined(_M_ARM)
 #include <arm_neon.h>
 
