lib/Lib.IntVector.Transpose.fst
@@ -11,6 +11,7 @@ let transpose4x4_uint32 #t vs =
   let v1' = vec_interleave_high v0 v1 in
   let v2' = vec_interleave_low v2 v3 in
   let v3' = vec_interleave_high v2 v3 in
+
   let v0'' = vec_interleave_low_n 2 v0' v2' in
   let v1'' = vec_interleave_high_n 2 v0' v2' in
   let v2'' = vec_interleave_low_n 2 v1' v3' in
@@ -36,22 +37,24 @@ let transpose8x8_uint32 #t vs =
   let v5' = vec_interleave_high v4 v5 in
   let v6' = vec_interleave_low v6 v7 in
   let v7' = vec_interleave_high v6 v7 in
-  let v0'' = vec_interleave_low_n 4 v0' v2' in
-  let v1'' = vec_interleave_high_n 4 v0' v2' in
-  let v2'' = vec_interleave_low_n 4 v1' v3' in
-  let v3'' = vec_interleave_high_n 4 v1' v3' in
-  let v4'' = vec_interleave_low_n 4 v4' v6' in
-  let v5'' = vec_interleave_high_n 4 v4' v6' in
-  let v6'' = vec_interleave_low_n 4 v5' v7' in
-  let v7'' = vec_interleave_high_n 4 v5' v7' in
-  let v0''' = vec_interleave_low_n 2 v0'' v4'' in
-  let v1''' = vec_interleave_high_n 2 v0'' v4'' in
-  let v2''' = vec_interleave_low_n 2 v1'' v5'' in
-  let v3''' = vec_interleave_high_n 2 v1'' v5'' in
-  let v4''' = vec_interleave_low_n 2 v2'' v6'' in
-  let v5''' = vec_interleave_high_n 2 v2'' v6'' in
-  let v6''' = vec_interleave_low_n 2 v3'' v7'' in
-  let v7''' = vec_interleave_high_n 2 v3'' v7'' in
+
+  let v0'' = vec_interleave_low_n 2 v0' v2' in
+  let v1'' = vec_interleave_high_n 2 v0' v2' in
+  let v2'' = vec_interleave_low_n 2 v1' v3' in
+  let v3'' = vec_interleave_high_n 2 v1' v3' in
+  let v4'' = vec_interleave_low_n 2 v4' v6' in
+  let v5'' = vec_interleave_high_n 2 v4' v6' in
+  let v6'' = vec_interleave_low_n 2 v5' v7' in
+  let v7'' = vec_interleave_high_n 2 v5' v7' in
+
+  let v0''' = vec_interleave_low_n 4 v0'' v4'' in
+  let v1''' = vec_interleave_high_n 4 v0'' v4'' in
+  let v2''' = vec_interleave_low_n 4 v1'' v5'' in
+  let v3''' = vec_interleave_high_n 4 v1'' v5'' in
+  let v4''' = vec_interleave_low_n 4 v2'' v6'' in
+  let v5''' = vec_interleave_high_n 4 v2'' v6'' in
+  let v6''' = vec_interleave_low_n 4 v3'' v7'' in
+  let v7''' = vec_interleave_high_n 4 v3'' v7'' in
   (v0''',v2''',v4''',v6''',v1''',v3''',v5''',v7''')
 
 
@@ -59,6 +62,87 @@ let transpose8x8 #t vs =
   match t with
   | U32 -> transpose8x8_uint32 #t vs
   | _ -> admit()
+
+
+val transpose16x16_uint32_lseq: #t:v_inttype{t == U32} -> vs:lseq (vec_t t 16) 16 -> lseq (vec_t t 16) 16
+let transpose16x16_uint32_lseq #t vs =
+  let (v0,v1,v2,v3,v4,v5,v6,v7) = (vs.[0],vs.[1],vs.[2],vs.[3],vs.[4],vs.[5],vs.[6],vs.[7]) in
+  let (v8,v9,v10,v11,v12,v13,v14,v15) = (vs.[8],vs.[9],vs.[10],vs.[11],vs.[12],vs.[13],vs.[14],vs.[15]) in
+
+  let v0' = vec_interleave_low v0 v1 in
+  let v1' = vec_interleave_high v0 v1 in
+  let v2' = vec_interleave_low v2 v3 in
+  let v3' = vec_interleave_high v2 v3 in
+  let v4' = vec_interleave_low v4 v5 in
+  let v5' = vec_interleave_high v4 v5 in
+  let v6' = vec_interleave_low v6 v7 in
+  let v7' = vec_interleave_high v6 v7 in
+  let v8' = vec_interleave_low v8 v9 in
+  let v9' = vec_interleave_high v8 v9 in
+  let v10' = vec_interleave_low v10 v11 in
+  let v11' = vec_interleave_high v10 v11 in
+  let v12' = vec_interleave_low v12 v13 in
+  let v13' = vec_interleave_high v12 v13 in
+  let v14' = vec_interleave_low v14 v15 in
+  let v15' = vec_interleave_high v14 v15 in
+
+  let v0'' = vec_interleave_low_n 2 v0' v2' in
+  let v2'' = vec_interleave_high_n 2 v0' v2' in
+  let v1'' = vec_interleave_low_n 2 v1' v3' in
+  let v3'' = vec_interleave_high_n 2 v1' v3' in
+  let v4'' = vec_interleave_low_n 2 v4' v6' in
+  let v6'' = vec_interleave_high_n 2 v4' v6' in
+  let v5'' = vec_interleave_low_n 2 v5' v7' in
+  let v7'' = vec_interleave_high_n 2 v5' v7' in
+  let v8'' = vec_interleave_low_n 2 v8' v10' in
+  let v10'' = vec_interleave_high_n 2 v8' v10' in
+  let v9'' = vec_interleave_low_n 2 v9' v11' in
+  let v11'' = vec_interleave_high_n 2 v9' v11' in
+  let v12'' = vec_interleave_low_n 2 v12' v14' in
+  let v14'' = vec_interleave_high_n 2 v12' v14' in
+  let v13'' = vec_interleave_low_n 2 v13' v15' in
+  let v15'' = vec_interleave_high_n 2 v13' v15' in
+
+  let v0' = vec_interleave_low_n 4 v0'' v4'' in
+  let v4' = vec_interleave_high_n 4 v0'' v4'' in
+  let v1' = vec_interleave_low_n 4 v1'' v5'' in
+  let v5' = vec_interleave_high_n 4 v1'' v5'' in
+  let v2' = vec_interleave_low_n 4 v2'' v6'' in
+  let v6' = vec_interleave_high_n 4 v2'' v6'' in
+  let v3' = vec_interleave_low_n 4 v3'' v7'' in
+  let v7' = vec_interleave_high_n 4 v3'' v7'' in
+  let v8' = vec_interleave_low_n 4 v8'' v12'' in
+  let v12' = vec_interleave_high_n 4 v8'' v12'' in
+  let v9' = vec_interleave_low_n 4 v9'' v13'' in
+  let v13' = vec_interleave_high_n 4 v9'' v13'' in
+  let v10' = vec_interleave_low_n 4 v10'' v14'' in
+  let v14' = vec_interleave_high_n 4 v10'' v14'' in
+
+  let v0 = vec_interleave_low_n 8 v0' v8' in
+  let v8 = vec_interleave_high_n 8 v0' v8' in
+  let v1 = vec_interleave_low_n 8 v1' v9' in
+  let v9 = vec_interleave_high_n 8 v1' v9' in
+  let v2 = vec_interleave_low_n 8 v2' v10' in
+  let v10 = vec_interleave_high_n 8 v2' v10' in
+  let v3 = vec_interleave_low_n 8 v3' v11' in
+  let v11 = vec_interleave_high_n 8 v3' v11' in
+  let v4 = vec_interleave_low_n 8 v4' v12' in
+  let v12 = vec_interleave_high_n 8 v4' v12' in
+  let v5 = vec_interleave_low_n 8 v5' v13' in
+  let v13 = vec_interleave_high_n 8 v5' v13' in
+  let v6 = vec_interleave_low_n 8 v6' v14' in
+  let v14 = vec_interleave_high_n 8 v6' v14' in
+  let v7 = vec_interleave_low_n 8 v7' v15' in
+  let v15 = vec_interleave_high_n 8 v7' v15' in
+
+  create16 v0 v2 v1 v3 v4 v6 v5 v7 v8 v10 v9 v11 v12 v14 v13 v15
+
+
+let transpose16x16_lseq #t vs =
+  match t with
+  | U32 -> transpose16x16_uint32_lseq #t vs
+  | _ -> admit()
+
 
 
 val transpose4x4_uint32_lemma_ij: #t:v_inttype{t == U32}
@@ -75,6 +159,7 @@ let transpose4x4_uint32_lemma_ij #t vs i j =
   vec_interleave_low_lemma_uint32_4 v2 v3;
   let v3' = vec_interleave_high v2 v3 in
   vec_interleave_high_lemma_uint32_4 v2 v3;
+
   let v0'' = vec_interleave_low_n 2 v0' v2' in
   vec_interleave_low_n_lemma_uint32_4_2 v0' v2';
   let v1'' = vec_interleave_high_n 2 v0' v2' in
@@ -102,7 +187,6 @@ val transpose8x8_uint32_lemma_ij: #t:v_inttype{t == U32}
   Lemma ((vec_v (transpose8x8_lseq vs).[i]).[j] == (vec_v vs.[j]).[i])
 
 let transpose8x8_uint32_lemma_ij #t vs i j =
-
   let (v0,v1,v2,v3,v4,v5,v6,v7) = (vs.[0],vs.[1],vs.[2],vs.[3],vs.[4],vs.[5],vs.[6],vs.[7]) in
   let v0' = vec_interleave_low v0 v1 in
   vec_interleave_low_lemma_uint32_8 v0 v1;
@@ -137,83 +221,83 @@ let transpose8x8_uint32_lemma_ij #t vs i j =
   let r7: lseq uint32 8 = create8 v6.(2) v7.(2) v6.(3) v7.(3) v6.(6) v7.(6) v6.(7) v7.(7) in
   assert (vec_v v7' == r7);
 
-  let v0'' = vec_interleave_low_n 4 v0' v2' in
-  vec_interleave_low_n_lemma_uint32_8_4 v0' v2';
+  let v0'' = vec_interleave_low_n 2 v0' v2' in
+  vec_interleave_low_n_lemma_uint32_8_2 v0' v2';
   let r0': lseq uint32 8 = create8 v0.(0) v1.(0) v2.(0) v3.(0) v0.(4) v1.(4) v2.(4) v3.(4) in
   assert (vec_v v0'' == r0');
 
-  let v1'' = vec_interleave_high_n 4 v0' v2' in
-  vec_interleave_high_n_lemma_uint32_8_4 v0' v2';
+  let v1'' = vec_interleave_high_n 2 v0' v2' in
+  vec_interleave_high_n_lemma_uint32_8_2 v0' v2';
   let r1': lseq uint32 8 = create8 v0.(1) v1.(1) v2.(1) v3.(1) v0.(5) v1.(5) v2.(5) v3.(5) in
   assert (vec_v v1'' == r1');
 
-  let v2'' = vec_interleave_low_n 4 v1' v3' in
-  vec_interleave_low_n_lemma_uint32_8_4 v1' v3';
+  let v2'' = vec_interleave_low_n 2 v1' v3' in
+  vec_interleave_low_n_lemma_uint32_8_2 v1' v3';
   let r2': lseq uint32 8 = create8 v0.(2) v1.(2) v2.(2) v3.(2) v0.(6) v1.(6) v2.(6) v3.(6) in
   assert (vec_v v2'' == r2');
 
-  let v3'' = vec_interleave_high_n 4 v1' v3' in
-  vec_interleave_high_n_lemma_uint32_8_4 v1' v3';
+  let v3'' = vec_interleave_high_n 2 v1' v3' in
+  vec_interleave_high_n_lemma_uint32_8_2 v1' v3';
   let r3': lseq uint32 8 = create8 v0.(3) v1.(3) v2.(3) v3.(3) v0.(7) v1.(7) v2.(7) v3.(7) in
   assert (vec_v v3'' == r3');
 
-  let v4'' = vec_interleave_low_n 4 v4' v6' in
-  vec_interleave_low_n_lemma_uint32_8_4 v4' v6';
+  let v4'' = vec_interleave_low_n 2 v4' v6' in
+  vec_interleave_low_n_lemma_uint32_8_2 v4' v6';
   let r4': lseq uint32 8 = create8 v4.(0) v5.(0) v6.(0) v7.(0) v4.(4) v5.(4) v6.(4) v7.(4) in
   assert (vec_v v4'' == r4');
 
-  let v5'' = vec_interleave_high_n 4 v4' v6' in
-  vec_interleave_high_n_lemma_uint32_8_4 v4' v6';
+  let v5'' = vec_interleave_high_n 2 v4' v6' in
+  vec_interleave_high_n_lemma_uint32_8_2 v4' v6';
   let r5': lseq uint32 8 = create8 v4.(1) v5.(1) v6.(1) v7.(1) v4.(5) v5.(5) v6.(5) v7.(5) in
   assert (vec_v v5'' == r5');
 
-  let v6'' = vec_interleave_low_n 4 v5' v7' in
-  vec_interleave_low_n_lemma_uint32_8_4 v5' v7';
+  let v6'' = vec_interleave_low_n 2 v5' v7' in
+  vec_interleave_low_n_lemma_uint32_8_2 v5' v7';
   let r6': lseq uint32 8 = create8 v4.(2) v5.(2) v6.(2) v7.(2) v4.(6) v5.(6) v6.(6) v7.(6) in
   assert (vec_v v6'' == r6');
 
-  let v7'' = vec_interleave_high_n 4 v5' v7' in
-  vec_interleave_high_n_lemma_uint32_8_4 v5' v7';
+  let v7'' = vec_interleave_high_n 2 v5' v7' in
+  vec_interleave_high_n_lemma_uint32_8_2 v5' v7';
   let r7': lseq uint32 8 = create8 v4.(3) v5.(3) v6.(3) v7.(3) v4.(7) v5.(7) v6.(7) v7.(7) in
   assert (vec_v v7'' == r7');
 
-  let v0''' = vec_interleave_low_n 2 v0'' v4'' in
-  vec_interleave_low_n_lemma_uint32_8_2 v0'' v4'';
+  let v0''' = vec_interleave_low_n 4 v0'' v4'' in
+  vec_interleave_low_n_lemma_uint32_8_4 v0'' v4'';
   let r0'': lseq uint32 8 = create8 v0.(0) v1.(0) v2.(0) v3.(0) v4.(0) v5.(0) v6.(0) v7.(0) in
   assert (vec_v v0''' == r0'');
 
-  let v1''' = vec_interleave_high_n 2 v0'' v4'' in
-  vec_interleave_high_n_lemma_uint32_8_2 v0'' v4'';
+  let v1''' = vec_interleave_high_n 4 v0'' v4'' in
+  vec_interleave_high_n_lemma_uint32_8_4 v0'' v4'';
   let r1'': lseq uint32 8 = create8 v0.(4) v1.(4) v2.(4) v3.(4) v4.(4) v5.(4) v6.(4) v7.(4) in
   assert (vec_v v1''' == r1'');
 
-  let v2''' = vec_interleave_low_n 2 v1'' v5'' in
-  vec_interleave_low_n_lemma_uint32_8_2 v1'' v5'';
+  let v2''' = vec_interleave_low_n 4 v1'' v5'' in
+  vec_interleave_low_n_lemma_uint32_8_4 v1'' v5'';
   let r2'': lseq uint32 8 = create8 v0.(1) v1.(1) v2.(1) v3.(1) v4.(1) v5.(1) v6.(1) v7.(1) in
   assert (vec_v v2''' == r2'');
 
-  let v3''' = vec_interleave_high_n 2 v1'' v5'' in
-  vec_interleave_high_n_lemma_uint32_8_2 v1'' v5'';
+  let v3''' = vec_interleave_high_n 4 v1'' v5'' in
+  vec_interleave_high_n_lemma_uint32_8_4 v1'' v5'';
   let r3'': lseq uint32 8 = create8 v0.(5) v1.(5) v2.(5) v3.(5) v4.(5) v5.(5) v6.(5) v7.(5) in
   assert (vec_v v3''' == r3'');
 
-  let v4''' = vec_interleave_low_n 2 v2'' v6'' in
-  vec_interleave_low_n_lemma_uint32_8_2 v2'' v6'';
+  let v4''' = vec_interleave_low_n 4 v2'' v6'' in
+  vec_interleave_low_n_lemma_uint32_8_4 v2'' v6'';
   let r4'': lseq uint32 8 = create8 v0.(2) v1.(2) v2.(2) v3.(2) v4.(2) v5.(2) v6.(2) v7.(2) in
   assert (vec_v v4''' == r4'');
 
-  let v5''' = vec_interleave_high_n 2 v2'' v6'' in
-  vec_interleave_high_n_lemma_uint32_8_2 v2'' v6'';
+  let v5''' = vec_interleave_high_n 4 v2'' v6'' in
+  vec_interleave_high_n_lemma_uint32_8_4 v2'' v6'';
   let r5'': lseq uint32 8 = create8 v0.(6) v1.(6) v2.(6) v3.(6) v4.(6) v5.(6) v6.(6) v7.(6) in
   assert (vec_v v5''' == r5'');
 
-  let v6''' = vec_interleave_low_n 2 v3'' v7'' in
-  vec_interleave_low_n_lemma_uint32_8_2 v3'' v7'';
+  let v6''' = vec_interleave_low_n 4 v3'' v7'' in
+  vec_interleave_low_n_lemma_uint32_8_4 v3'' v7'';
   let r6'': lseq uint32 8 = create8 v0.(3) v1.(3) v2.(3) v3.(3) v4.(3) v5.(3) v6.(3) v7.(3) in
   assert (vec_v v6''' == r6'');
 
-  let v7''' = vec_interleave_high_n 2 v3'' v7'' in
-  vec_interleave_high_n_lemma_uint32_8_2 v3'' v7'';
+  let v7''' = vec_interleave_high_n 4 v3'' v7'' in
+  vec_interleave_high_n_lemma_uint32_8_4 v3'' v7'';
   let r7'': lseq uint32 8 = create8 v0.(7) v1.(7) v2.(7) v3.(7) v4.(7) v5.(7) v6.(7) v7.(7) in
   assert (vec_v v7''' == r7'');
   let res = create8 v0''' v2''' v4''' v6''' v1''' v3''' v5''' v7''' in
@@ -224,3 +308,5 @@ let transpose8x8_lemma #t vs =
   match t with
   | U32 -> Classical.forall_intro_2 (transpose8x8_uint32_lemma_ij vs)
   | _ -> admit()
+
+let transpose16x16_lemma #t vs = admit()
