lib/Lib.IntVector.Transpose.fsti
@@ -33,8 +33,14 @@ let transpose8x8_lseq (#t:v_inttype) (vs:lseq (vec_t t 8) 8) : lseq (vec_t t 8) 
   let (r0,r1,r2,r3,r4,r5,r6,r7) = transpose8x8 (v0,v1,v2,v3,v4,v5,v6,v7) in
   create8 r0 r1 r2 r3 r4 r5 r6 r7
 
+val transpose16x16_lseq: #t:v_inttype -> vs:lseq (vec_t t 16) 16 -> lseq (vec_t t 16) 16
+
+
 val transpose4x4_lemma: #t:v_inttype -> vs:lseq (vec_t t 4) 4 ->
   Lemma (forall (i:nat{i < 4}) (j:nat{j < 4}). (vec_v (transpose4x4_lseq vs).[i]).[j] == (vec_v vs.[j]).[i])
 
 val transpose8x8_lemma: #t:v_inttype -> vs:lseq (vec_t t 8) 8 ->
   Lemma (forall (i:nat{i < 8}) (j:nat{j < 8}). (vec_v (transpose8x8_lseq vs).[i]).[j] == (vec_v vs.[j]).[i])
+
+val transpose16x16_lemma: #t:v_inttype -> vs:lseq (vec_t t 16) 16 ->
+  Lemma (forall (i:nat{i < 16}) (j:nat{j < 16}). (vec_v (transpose16x16_lseq vs).[i]).[j] == (vec_v vs.[j]).[i])
